spvspv proof progress

SV.v
@@ -24,13 +24,75 @@ Section pure_facts.
 Import List.
 
 Definition sorted (l : list int) : Prop. Admitted.
+Definition max (l : list int) : int. Admitted.
 
+Definition merge (l1 l2 : list int) : list int. Admitted.
+
+Lemma In_merge l1 l2 x : In x (merge l1 l2) = (In x l1 \/ In x l2).
+Proof. Admitted.
+
+Lemma sorted_nodup l : sorted l -> NoDup l.
+Admitted.
+
+Lemma sorted_merge l1 l2 : sorted l1 -> sorted l2 -> sorted (merge l1 l2).
+Admitted.
+
+Lemma sorted_max_size l i : 
+  i + 1 = length l -> l[i] = max l.
+Admitted.
+
+Lemma max_sublist l1 l2 : 
+  (forall x, In x l1 -> In x l2) -> max l2 >= max l1.
+Admitted.
+
+Lemma nth_le_max l i :
+  i >= 0 ->
+  sorted l ->
+  l[i] >= max l -> i + 1 = length l.
+Admitted.
+
+Lemma sorted_le i j l :
+  sorted l ->
+  0 <= i < length l ->
+  0 <= j < length l ->
+    i < j -> l[i] < l[j].
+Admitted.
+
+Lemma max_takeS i l : 
+  0 <= i < length l ->
+  max (take (abs (i + 1)) l) = Z.max l[i] (max (take (abs i) l)).
+Admitted.
+
+Lemma In_lt x i l :
+  0 <= i < length l - 1 ->
+  sorted l ->
+    In x l -> x < l[i+1] -> x <= l[i].
+Admitted.
+
+Lemma max_le x l : 
+  In x l -> x <= max l.
+Proof.
+Admitted.
+
+Lemma size_merge l1 l2: 
+  length (merge l1 l2) >= Z.max (length l1) (length l2).
+Proof.
+Admitted.
+
+Lemma max0 : max nil = -1.
+Proof.
+Admitted.
+
+Lemma In_le_0 l x :
+  sorted l -> In x l -> x >= l[0].
+Admitted.
 
 End pure_facts.
 
 Module sparse_vec.
 
-Module Export AD := WithUnary(IntDom).
+(* Module Export AD := WithUnary(IntDom). *)
+Import coo_vec.
 
 Notation "H1 '\\*' H2" := (hstar H1 H2)
   (at level 42, right associativity, format "H1  \\* '//' H2") : hprop_scope.
@@ -58,8 +120,6 @@ Hypothesis sorted_yind : sorted yind.
 Hypothesis xind_leq : forall x, In x xind -> 0 <= x < M.
 Hypothesis yind_leq : forall x, In x yind -> 0 <= x < M.
 
-Definition get := coo_vec.get.
-
 Notation "'while' C '{' T '}'"  :=
   (While C T)
   (in custom trm at level 69,
@@ -68,34 +128,62 @@ Notation "'while' C '{' T '}'"  :=
 
 Definition dotprod := <{
   fun xind xval yind yval =>
-    let ans = 0 in
+    let ans = ref 0 in
     let iX = ref 0 in 
     let iY = ref 0 in 
-    let "iXl" = iX < Nx in 
-    let "iYl" = iY < Ny in
-    let "cnd" = "iXl" && "iYl" in 
-      while "cnd" {
-        let "iXind" = xind[iX] in 
-        let "iYind" = yind[iY] in 
+      while (
+        let "ix" = !iX in
+        let "iy" = !iY in
+        let "iXl" = "ix" < Nx in 
+        let "iYl" = "iy" < Ny in
+        "iXl" && "iYl") {
+        let "ix" = !iX in
+        let "iy" = !iY in
+        let "iXind" = xind["ix"] in 
+        let "iYind" = yind["iy"] in 
         let "cnd" = "iXind" = "iYind" in 
         if "cnd" then 
-          let "iXind" = xval[iX] in 
-          let "iYind" = yval[iY] in 
+          let "iXind" = xval["ix"] in 
+          let "iYind" = yval["iy"] in 
           let "val" = "iXind" * "iYind" in
           ans += "val";
           ++iX;
           ++iY
         else 
-          let "cnd" = "iXl" < "iYl" in 
+          let "cnd" = "iXind" < "iYind" in 
           if "cnd" then 
             ++iX 
           else ++iY
-      }; ans
+      }; !ans
 }>.
 
+Hint Rewrite hstar_fset_Lab : hstar_fset.
+
+Definition arr1 x_ind y_ind x_val y_val := arr(x_ind, xind)⟨1, 0⟩ \* arr(y_ind, yind)⟨1, 0⟩ \*
+  arr(x_val, xval)⟨1, 0⟩ \* arr(y_val, yval)⟨1, 0⟩.
+
+Ltac fold' := 
+  rewrite ?label_single ?wp_single
+    -/(While_aux _ _) 
+    -/(While _ _) //=.
+
+Notation size := Datatypes.length.
+
+Lemma not_isTrueE (P: Prop) : (~ isTrue P) = ~ P.
+Proof.
+Admitted.
+
+Ltac bool_rew := 
+  rewrite ?false_eq_isTrue_eq ?istrue_isTrue_eq ?true_eq_isTrue_eq -?(isTrue_and, isTrue_not, isTrue_or) ?not_isTrueE.
+
+Lemma val_int_eq i j : 
+  (val_int i = val_int j) = (i = j).
+Proof. by extens; split=> [[]|]->. Qed.
+
+Transparent take.
+
 Lemma dotprod_spec `{Inhab D} (x_ind x_val y_ind y_val : loc) : 
-  {{ arr(x_ind, xind)⟨1, 0⟩ \* arr(y_ind, yind)⟨1, 0⟩ \*
-     arr(x_val, xval)⟨1, 0⟩ \* arr(y_val, yval)⟨1, 0⟩ \\*
+  {{ arr1 x_ind y_ind x_val y_val \*
      (\*_(i <- `[0, M]) arr(x_ind, xind)⟨2, i⟩) \\*
      (\*_(i <- `[0, M]) arr(x_val, xval)⟨2, i⟩) \\* 
      (\*_(i <- `[0, M]) arr(y_ind, yind)⟨3, i⟩) \\*
@@ -106,9 +194,199 @@ Lemma dotprod_spec `{Inhab D} (x_ind x_val y_ind y_val : loc) :
     [3| ld in `[0,M] => get Ny ld y_ind y_val]
   }]
   {{ hv, \[hv[`1](0) = Σ_(i <- `[0,M]) (hv[`2](i) * hv[`3](i))] \* \Top}}.
-Proof.
+Proof with fold'.
+  set (ind := merge xind yind).
+  have?: NoDup xind by exact/sorted_nodup.
+  have?: NoDup yind by exact/sorted_nodup.
+  have?: NoDup ind by exact/sorted_nodup/sorted_merge.
+  xfocus (2,0) (ind).
+  rewrite {1 2}(hbig_fset_part `[0, M] ind).
+  xapp (@get_spec_out xind xval); eauto.
+  { case=> ??/=/[!@indom_label_eq]-[_].
+    rewrite /intr filter_indom/= /Sum.mem/ind In_merge; autos*. }
+  set (H1 := hbig_fset hstar (_ ∖ _) _); 
+  set (H2 := hbig_fset hstar (_ ∖ _) _).
+  xframe (H1 \* H2); clear H1 H2.
+  xfocus (3,0) (ind).
+  rewrite (hbig_fset_part `[0, M] ind).
+  xapp (@get_spec_out yind yval); eauto.
+  { case=> ??/=/[!@indom_label_eq]-[_].
+    rewrite /intr filter_indom/= /Sum.mem/ind In_merge; autos*. }
+  set (H1 := hbig_fset hstar (_ ∖ _) _); 
+  set (H2 := hbig_fset hstar (_ ∖ _) _).
+  xframe (H1 \* H2); clear H1 H2.
+  set (H1 := _ \* hbig_fset _ _ _); set (H2 := _ \* H1); set (arrs := _ \* H2).
+  xin (1,0) : xwp; xapp=> ans; xwp; xapp=> iX; xwp; xapp=> iY...
+  have E : `[0,M] ∩ ind = ind.
+  { apply/fset_extens=> ?. 
+    rewrite /intr filter_indom /ind -fset_of_list_in /Sum.mem ?In_merge; splits*.
+    rewrite ?indom_interval=> -[]; autos*. }
+  rewrite ?E (fset_of_list_nodup 0) //.
+  set (cond ix iy := isTrue (ix < Nx /\ iy < Ny)).
+  set (Inv (b : bool) (i : int) := 
+    \exists (ix iy : int), 
+      iY ~⟨(1, 0)%Z, 0⟩~> iy \* iX ~⟨(1, 0)%Z, 0⟩~> ix \*
+      arr1 x_ind y_ind x_val y_val \*
+      \[(i = size ind -> ~ b) /\ 0 <= ix /\ 0 <= iy /\
+        (i < size ind -> ind[i] > max (take (abs ix) xind)) /\
+        (i < size ind -> ind[i] > max (take (abs iy) yind)) /\ 
+        b = cond ix iy /\
+        (b -> 
+          (ind[i] = Z.min xind[ix] yind[iy] /\ 
+          (forall x, In x xind -> x < xind[ix] -> x < yind[iy]) /\  
+          (forall y, In y yind -> y < yind[iy] -> y < xind[ix])))]).
+  set (op hv i := hv[`2](ind[i]) * hv[`3](ind[i])).
+  set (R1 i := arr(y_ind, yind)⟨3,i⟩ \* arr(y_val, yval)⟨3,i⟩).
+  set (R2 i := arr(x_ind, xind)⟨2,i⟩ \* arr(x_val, xval)⟨2,i⟩).
+  eapply xwhile_big_op_lemma2 with 
+    (Inv := Inv) (op := op) 
+    (R1 := R1) (R2 := R2) 
+    (R1' := fun=> \Top) (R2':= fun=> \Top) (p := ans)=> //; try eassumption.
+  { move=> l s ?.
+    rewrite {1}/Inv; xnsimpl=> ix iy[?][?][?][LM1][LM2][].
+    rewrite /cond. bool_rew=> -[??]/(_ eq_refl)-[]indlE[L1 L2].
+    rewrite /arr1; clear arrs H1 H2.
+    xin (1,0): do 5 (xwp; xapp); xwp; xif=> C.
+    { xin (1,0): do 3 (xwp; xapp); xwp; xapp incr.spec; (xwp; xapp incr1.spec); xapp incr1.spec=> ?.
+      rewrite /op /=; rewrite <-?hstar_assoc.
+      set (Heap := _ \* harray_int xind _ _); rewrite /R2...
+      rewrite val_int_eq in C; rewrite {-1 4}indlE -C Z.min_id.
+      xin (2,0): fold'; xapp get_spec_in; eauto.
+      rewrite /R1 indlE C Z.min_id...
+      xapp get_spec_in; eauto.
+      rewrite /Heap /Inv /arr1/cond.
+      have SlE: l + 1 = size ind -> ~ isTrue (ix + 1 < Nx /\ iy + 1 < Ny). 
+      { move: C indlE=>-> /[! Z.min_id]/[swap]/sorted_max_size->; bool_rew.
+        have: max ind >= max yind by apply/max_sublist=>?; rewrite In_merge; right.
+        move=>/[swap]->/nth_le_max-> //; lia. }
+      xsimpl (ix + 1) (iy + 1); splits; [|lia|lia| | |autos*|]...
+      { move=> ?; rewrite max_takeS; last lia. 
+        suff: ind[l] < ind[l+1] by lia.
+        apply/sorted_le; autos*; try lia.
+        exact/sorted_merge. }
+      { move=> ?; rewrite max_takeS; last lia. 
+        suff: ind[l] < ind[l+1] by lia.
+        apply/sorted_le; autos*; try lia.
+        exact/sorted_merge. }
+      bool_rew=> -[]??; splits*.
+      { admit. }
+      { move=> x ??; move: (@sorted_le iy (iy+1) yind sorted_yind).
+        suff: (x <= xind[ix]) by lia.
+        apply/In_lt... lia. }
+      move=> x ??; move: (@sorted_le ix (ix+1) xind sorted_xind).
+      suff: (x <= yind[iy]) by lia.
+      apply/In_lt... lia. }
+    rewrite /op.
+    xin (1,0): xwp; xapp; xwp; xif=> L; xapp incr1.spec=> ?.
+    { rewrite /op /=; rewrite <-?hstar_assoc.
+      set (Heap := _ \* harray_int yval _ _); rewrite /R2...
+      rewrite indlE Z.min_l; last lia.
+      xin (2,0): fold'; xapp get_spec_in...
+      rewrite /R1; xapp get_spec_out_unary; eauto.
+      { move/L2/(_ L); lia. }
+      rewrite Z.mul_0_r Z.add_0_r.
+      rewrite /Heap /Inv /arr1/cond. 
+      xsimpl (ix + 1) (iy); splits; [|lia|lia| | |autos*|].
+      { move: indlE=> /[!Z.min_l] //; last lia. 
+        move=>/[swap]/sorted_max_size->; bool_rew.
+        have: max ind >= max xind by apply/max_sublist=>?; rewrite In_merge; left.
+        move=>/[swap]->/nth_le_max-> //; lia. }
+      { move=> ?; rewrite max_takeS; last lia. 
+        suff: ind[l] < ind[l+1] by lia.
+        apply/sorted_le; autos*; try lia.
+        exact/sorted_merge. }
+      { move=> ?. suff: ind[l] < ind[l+1] by lia.
+        apply/sorted_le; autos*; try lia.
+        exact/sorted_merge. }
+      bool_rew=> -[]??; splits*.
+      { admit. }
+      { move=> x ??; move: (@sorted_le ix (ix+1) xind sorted_xind)=> ?.
+        suff: (x <= xind[ix]) by lia.
+        apply/In_lt... lia. }
+      move=> ? /L2/[apply].
+      move: (@sorted_le ix (ix+1) xind sorted_xind); lia. }
+    rewrite /op /=; rewrite <-?hstar_assoc.
+    set (Heap := _ \* harray_int yval _ _); rewrite /R1...
+    rewrite indlE Z.min_r; last lia.
+    xin (3,0): fold'; xapp get_spec_in...
+    rewrite /R2; xapp get_spec_out_unary; eauto.
+    { move/L1. rewrite val_int_eq in C; lia. }
+    rewrite Z.mul_0_l Z.add_0_r.
+    rewrite /Heap /Inv /arr1/cond; xsimpl (ix) (iy+1); splits; [|lia|lia| | |autos*|].
+    { move: indlE=> /[!Z.min_r] //; last lia. 
+      move=>/[swap]/sorted_max_size->; bool_rew.
+      have: max ind >= max yind by apply/max_sublist=>?; rewrite In_merge; right.
+      move=>/[swap]->/nth_le_max-> //; lia. }
+    { move=> ?. suff: ind[l] < ind[l+1] by lia.
+      apply/sorted_le; autos*; try lia.
+      exact/sorted_merge. }
+    { move=> ?; rewrite max_takeS; last lia. 
+      suff: ind[l] < ind[l+1] by lia.
+      apply/sorted_le; autos*; try lia.
+      exact/sorted_merge. }
+    bool_rew=> -[]??; splits*.
+    { admit. }
+    { move=> ? /L1/[apply].
+      move: (@sorted_le iy (iy+1) yind sorted_yind); lia. }
+    rewrite val_int_eq in C.
+    move=> x ??; move: (@sorted_le iy (iy+1) yind sorted_yind)=> ?.
+    suff: (x <= yind[iy]) by lia.
+    apply/In_lt... lia. }
+  { move=> l *; rewrite /Inv/op/ntriple.
+    xpull=> ix iy []_[]?[]?[]L1[]L2; rewrite /cond; bool_rew=> /[!not_and_eq]-[] []G _.
+    { rewrite /R1.
+      xin (3,0): fold'; xapp get_spec=> *...
+      rewrite /R2.
+      xapp get_spec_out_unary...
+      { move/max_le; move: L1; rewrite take_ge ?length_List_length; (math||lia). }
+      splits*=> //.
+      { move=> ?. suff: ind[l] < ind[l+1] by lia.
+        apply/sorted_le; autos*; try lia.
+        exact/sorted_merge. }
+      { move=> ?. suff: ind[l] < ind[l+1] by lia.
+        apply/sorted_le; autos*; try lia.
+        exact/sorted_merge. }
+        bool_rew; lia. }
+    rewrite /R2.
+    xin (2,0): fold'; xapp get_spec=> *...
+    rewrite /R1.
+    xapp get_spec_out_unary...
+    { move/max_le; move: L2; rewrite take_ge ?length_List_length; (math||lia). }
+    { lia. }
+    splits*=> //.
+    { move=> ?. suff: ind[l] < ind[l+1] by lia.
+      apply/sorted_le; autos*; try lia.
+      exact/sorted_merge. }
+    { move=> ?. suff: ind[l] < ind[l+1] by lia.
+      apply/sorted_le; autos*; try lia.
+      exact/sorted_merge. }
+    bool_rew; lia. }
+  { move=> ???. rewrite /ntriple -xnwp1_lemma /=.
+    rewrite /Inv; xpull=> ix iy C.
+    do ? (xwp; xapp). xapp and.spec=> //.
+    by move=> ?->; bool_rew; case: C=> ? [?][?][?][?][]->. }
+  { move=> b; rewrite /Inv; xsimpl*=> ?? []/(_ eq_refl); by case: b. }
+  { admit. }
+  { admit. }
+  { admit. }
+  { lia. }
+  { rewrite /arr1 /Inv/arrs/arr1; xsimpl 0 0.
+    { splits; [|lia|lia| | |autos*|].
+      { rewrite /cond/ind; bool_rew; move: (size_merge xind yind); lia. }
+        { rewrite abs_0 /= max0=> ?.
+          have: (In (nth 0 ind 0) ind) by apply/nth_In; lia.
+          rewrite In_merge=> -[/xind_leq|/yind_leq]; lia. }
+        { rewrite abs_0 /= max0=> ?.
+          have: (In (nth 0 ind 0) ind) by apply/nth_In; lia.
+          rewrite In_merge=> -[/xind_leq|/yind_leq]; lia. }
+        do ? split.
+        { admit. }
+        { move=> ?/(In_le_0 _ sorted_xind); lia. }
+        move=> ?/(In_le_0 _ sorted_yind); lia. }
+    rewrite /H2/H1 ?E (fset_of_list_nodup 0) // /R1 /R2.
+    rewrite -> ?hbig_fset_hstar; xsimpl*. }
+  simpl=> v. xapp; xsimpl; rewrite /op.
 Admitted.
-
 
 End sparse_vec.
 
